Make naming more consistent in the memory model

src/lang/memory.v
@@ -24,7 +24,7 @@ Instance thread_view_bottom : Bottom thread_view := ε.
 
 Notation store_view tv := (tv.1).1.
 Notation flush_view tv := (tv.1).2.
-Notation wb_buffer_view tv := (tv.2).
+Notation buffer_view tv := (tv.2).
 
 Notation history := (gmap time message).
 
@@ -41,9 +41,9 @@ Section consistent_cut.
   Definition discard_msg_views (msg : message) : message :=
     Msg msg.(msg_val) ∅ ∅ ∅.
 
-  (* For each location in [p] pick the message in the store that it specifies. *)
-  Definition slice_of_store (p : view) (σ : store) : store :=
-    (λ (hist : gmap _ _), discard_msg_views <$> hist) <$> (slice_of_hist p σ).
+  (* For each location in [V] pick the message in the store that it specifies. *)
+  Definition slice_of_store (V : view) (σ : store) : store :=
+    (λ (hist : gmap _ _), discard_msg_views <$> hist) <$> (slice_of_hist V σ).
 
   Definition consistent_cut (CV : view) (σ : store) : Prop :=
     map_Forall
@@ -68,10 +68,10 @@ Section consistent_cut.
     done.
   Qed.
 
-  (* if [p] is a consistent cut of [σ] then the domain of [p] is included in
+  (* if [V] is a consistent cut of [σ] then the domain of [V] is included in
   [σ]. Intuitively, the recovered locations where all in the heap. *)
-  Lemma consistent_cut_subseteq_dom p σ :
-    consistent_cut p σ → dom (gset _) p ⊆ dom _ σ.
+  Lemma consistent_cut_subseteq_dom V σ :
+    consistent_cut V σ → dom (gset _) V ⊆ dom _ σ.
   Proof.
     rewrite /consistent_cut.
     intros map.
@@ -181,7 +181,7 @@ End consistent_cut.
 
 Section memory.
 
-  Implicit Types (v : val) (ℓ : loc) (σ : store) (p : view).
+  Implicit Types (v : val) (ℓ : loc) (σ : store) (V : view).
 
   Inductive mem_event : Type :=
   | MEvAllocN (a : memory_access) ℓ (len : nat) v
@@ -213,7 +213,9 @@ Section memory.
 
   Lemma heap_array_lookup ℓ a SV PV (vs : list val) (ow : history) (k : loc) :
     (heap_array ℓ a SV PV vs : store) !! k = Some ow ↔
-    ∃ j w, (0 ≤ j)%Z ∧ k = ℓ +ₗ j ∧ (ow = initial_history a SV PV w) ∧ vs !! (Z.to_nat j) = (Some w).
+    ∃ j w, (0 ≤ j)%Z ∧ k = ℓ +ₗ j ∧
+            (ow = initial_history a SV PV w) ∧
+            vs !! (Z.to_nat j) = (Some w).
   Proof.
     revert k ℓ; induction vs as [|v' vs IH]=> l' ℓ /=.
     { rewrite lookup_empty. naive_solver lia. }
@@ -249,88 +251,87 @@ Section memory.
 
   Inductive mem_step : mem_config → thread_view → mem_event → mem_config → thread_view → Prop :=
   (* Allocating a new location. *)
-  | MStepAllocN a σ SV PV BV ℓ (len : nat) v p :
-     (0 < len)%Z → (* (∀ i, (0 ≤ i)%Z → (i < n)%Z → σ.(heap) !! (ℓ +ₗ i) = None) → *)
+  | MStepAllocN a σ SV FV BV ℓ (len : nat) v PV :
+     (0 < len)%Z →
      (∀ idx, (0 ≤ idx)%Z → (idx < len)%Z → σ !! (ℓ +ₗ idx) = None) → (* This is a fresh segment of the heap not already in use. *)
      (* V' = <[ ℓ := 0 ]>SV → (* V' incorporates the new event in the threads view. *) This may not be needed. *)
-     mem_step (σ, p) (SV, PV, BV)
+     mem_step (σ, PV) (SV, FV, BV)
               (MEvAllocN a ℓ len v)
-              (state_init_heap a ℓ len SV PV v σ, p) (SV, PV, BV)
+              (state_init_heap a ℓ len SV FV v σ, PV) (SV, FV, BV)
   (* A normal non-atomic load. *)
-  | MStepLoad (σ : store) SV PV BV t (ℓ : loc) (v : val) h p :
+  | MStepLoad (σ : store) SV FV BV t (ℓ : loc) (v : val) h PV :
      σ !! ℓ = Some h →
      msg_val <$> (h !! t) = Some v →
-     (SV !!0 ℓ) ≤ t →
-     mem_step (σ, p) (SV, PV, BV)
+     SV !!0 ℓ ≤ t →
+     mem_step (σ, PV) (SV, FV, BV)
               (MEvLoad ℓ v)
-              (σ, p) (SV, PV, BV)
-              (* (σ, p) ((<[ ℓ := t ]>SV), PV, BV) (* This variant includes the timestamp of the loaded msg. *) *)
+              (σ, PV) (SV, FV, BV)
+              (* (σ, PV) ((<[ ℓ := t ]>SV), FV, BV) (* This variant includes the timestamp of the loaded msg. *) *)
   (* An atomic acquire load. *)
-  | MStepLoadAcquire σ SV PV BV t ℓ (v : val) MV MP _MP h p :
+  | MStepLoadAcquire σ SV FV BV t ℓ (v : val) MV MP _MP h PV :
      σ !! ℓ = Some h →
-     (h !! t) = Some (Msg v MV MP _MP) →
-     (SV !!0 ℓ) ≤ t →
-     mem_step (σ, p) (SV, PV, BV)
+     h !! t = Some (Msg v MV MP _MP) →
+     SV !!0 ℓ ≤ t →
+     mem_step (σ, PV) (SV, FV, BV)
               (MEvLoadAcquire ℓ v)
-              (σ, p) (SV ⊔ MV, PV, BV ⊔ MP) (* An acquire incorporates both the store view and the persistent view. *)
+              (σ, PV) (SV ⊔ MV, FV, BV ⊔ MP) (* An acquire incorporates both the store view and the persistent view. *)
   (* A normal non-atomic write. *)
-  | MStepStore σ SV PV BV t ℓ (v : val) h V' p :
+  | MStepStore σ SV FV BV t ℓ (v : val) h V' PV :
      σ !! ℓ = Some h →
-     (h !! t) = None → (* No event exists at t already. *)
-     (SV !!0 ℓ) < t →
+     h !! t = None → (* No event exists at t already. *)
+     SV !!0 ℓ < t →
      V' = <[ℓ := MaxNat t]>SV → (* V' incorporates the new event in the threads view. *)
-     mem_step (σ, p) (SV, PV, BV)
+     mem_step (σ, PV) (SV, FV, BV)
              (MEvStore ℓ v)
-             (<[ℓ := <[t := Msg v ∅ ∅ PV]>h]>σ, p) (V', PV, BV)
+             (<[ℓ := <[t := Msg v ∅ ∅ FV]>h]>σ, PV) (V', FV, BV)
   (* An atomic release write. *)
-  | MStepStoreRelease σ SV PV BV t ℓ (v : val) h V' p :
+  | MStepStoreRelease σ SV FV BV t ℓ (v : val) h V' PV :
      σ !! ℓ = Some h →
-     (h !! t) = None → (* No event exists at t already. *)
-     (SV !!0 ℓ) < t →
+     h !! t = None → (* No event exists at t already. *)
+     SV !!0 ℓ < t →
      V' = <[ℓ := MaxNat t]>SV → (* V' incorporates the new event in the threads view. *)
-     mem_step (σ, p) (SV, PV, BV)
+     mem_step (σ, PV) (SV, FV, BV)
               (MEvStoreRelease ℓ v)
-              (<[ℓ := <[t := Msg v V' PV PV]>h]>σ, p) (V', PV, BV) (* A release releases both V' and PV. *)
+              (<[ℓ := <[t := Msg v V' FV FV]>h]>σ, PV) (V', FV, BV) (* A release releases both V' and FV. *)
   (* Read-modify-write instructions. *)
-  | MStepRMW σ ℓ h v MV MP SV t S' PV P' BV p v' _MP :
+  | MStepRMW σ ℓ h v MV MP SV t SV' FV P' BV PV v' _MP :
      σ !! ℓ = Some h →
-     (SV !!0 ℓ) ≤ t →
-     (h !! t) = Some (Msg v MV MP _MP) → (* We read an event at time [t]. *)
+     SV !!0 ℓ ≤ t →
+     h !! t = Some (Msg v MV MP _MP) → (* We read an event at time [t]. *)
      (* All values that we could have reads are comparable to [v]. *)
      (∀ t' msg, SV !!0 ℓ ≤ t' → h !! t' = Some msg → vals_compare_safe msg.(msg_val) v) →
-     (h !! (t + 1)) = None → (* The next timestamp is available, ensures that no other RMW read this event. *)
-     S' = (<[ ℓ := MaxNat (t + 1) ]>(SV ⊔ MV)) → (* S' incorporates the new event in the threads view. *)
-     P' = PV ⊔ MP →
-     mem_step (σ, p) (SV, PV, BV)
+     h !! (t + 1) = None → (* The next timestamp is available, ensures that no other RMW read this event. *)
+     SV' = (<[ ℓ := MaxNat (t + 1) ]>(SV ⊔ MV)) → (* SV' incorporates the new event in the threads view. *)
+     P' = FV ⊔ MP →
+     mem_step (σ, PV) (SV, FV, BV)
               (MEvRMW ℓ v v')
-              (<[ℓ := <[t + 1 := Msg v S' P' P']>h]>σ, p) (S', PV, BV ⊔ MP)
-  | MStepRMWFail σ SV PV BV t ℓ (v_i v_t : val) MV MP _MP h p :
+              (<[ℓ := <[t + 1 := Msg v SV' P' P']>h]>σ, PV) (SV', FV, BV ⊔ MP)
+  | MStepRMWFail σ SV FV BV t ℓ (v_i v_t : val) MV MP _MP h PV :
      σ !! ℓ = Some h →
-     (h !! t) = Some (Msg v_t MV MP _MP) →
-     (SV !!0 ℓ) ≤ t →
+     h !! t = Some (Msg v_t MV MP _MP) →
+     SV !!0 ℓ ≤ t →
      (* All values that we could have reads are comparable to [v_t]. *)
      (∀ t' msg, SV !!0 ℓ ≤ t' → h !! t' = Some msg → vals_compare_safe msg.(msg_val) v_i) →
      (h !! (t + 1)) = None →
-     mem_step (σ, p) (SV, PV, BV)
+     mem_step (σ, PV) (SV, FV, BV)
               (MEvRMWFail ℓ v_i v_t)
-              (σ, p) (SV ⊔ MV, PV, BV ⊔ MP) (* An acquire incorporates both the store view and the persistent view. *)
+              (σ, PV) (SV ⊔ MV, FV, BV ⊔ MP) (* An acquire incorporates both the store view and the persistent view. *)
   (* Write-back instruction. *)
-  | MStepFlush σ SV PV BV ℓ t p :
-     (* σ !! ℓ = Some h → *)
-     (SV !!0 ℓ) = t → (* An equality here is fine, the timestamps are only lower bounds anyway. *)
-     mem_step (σ, p) (SV, PV, BV)
+  | MStepFlush σ SV FV BV ℓ t PV :
+     SV !!0 ℓ = t → (* An equality here is fine, the timestamps are only lower bounds anyway. *)
+     mem_step (σ, PV) (SV, FV, BV)
               (MEvFlush ℓ)
-              (σ, p) (SV, PV, {[ℓ := MaxNat t]} ⊔ BV)
+              (σ, PV) (SV, FV, {[ℓ := MaxNat t]} ⊔ BV)
   (* Asynchronous fence. *)
-  | MStepFence σ SV PV BV p :
-     mem_step (σ, p) (SV, PV, BV)
+  | MStepFence σ SV FV BV PV :
+     mem_step (σ, PV) (SV, FV, BV)
               MEvFence
-              (σ, p) (SV, PV ⊔ BV, BV)
+              (σ, PV) (SV, FV ⊔ BV, BV)
   (* Synchronous fence. *)
-  | MStepFenceSync σ SV PV BV p :
-     mem_step (σ, p) (SV, PV, BV)
+  | MStepFenceSync σ SV FV BV PV :
+     mem_step (σ, PV) (SV, FV, BV)
               MEvFenceSync
-              (σ, p ⊔ BV) (SV, PV ⊔ BV, BV).
+              (σ, PV ⊔ BV) (SV, FV ⊔ BV, BV).
 
   (* The crash step is different from the other steps in that it does not depend
   on any current thread. We therefore define it as a separate type. *)
@@ -341,12 +342,12 @@ Section memory.
      crash_step (σ, p) (slice_of_store p' σ, view_to_zero p').
 
   (* It is always possible to allocate a section of memory. *)
-  Lemma alloc_fresh v (len : nat) a σ p SV PV BV :
+  Lemma alloc_fresh v (len : nat) a σ p SV FV BV :
     let ℓ := fresh_locs (dom (gset loc) σ) in (* ℓ is directly after the largest allocated location. *)
     (0 < len)%Z →
-    mem_step (σ, p) (SV, PV, BV)
+    mem_step (σ, p) (SV, FV, BV)
              (MEvAllocN a ℓ len v)
-             (state_init_heap a ℓ len SV PV v σ, p) (SV, PV, BV).
+             (state_init_heap a ℓ len SV FV v σ, p) (SV, FV, BV).
   Proof.
     intros. apply MStepAllocN; first done.
     intros. apply not_elem_of_dom.
